module Lambda where

open import Relation.Binary.PropositionalEquality using (_≡_; _≢_; refl)
open import Data.String using (String; _≟_)
open import Data.Nat using (ℕ; zero; suc)
open import Data.Empty using (⊥; ⊥-elim)
open import Relation.Nullary using (Dec; yes; no; ¬_)
open import Data.List using (List; _∷_; [])
open import Data.Product using (_×_; proj₁; proj₂) renaming (_,_ to ⟨_,_⟩)
open import Isomorphism using (_≲_; _≃_; extensionality)

Id : Set
Id = String

infix  5  ƛ_⇒_
infix  5  μ_⇒_
infixl 7  _∙_
infix  8  `suc_
infix  9  `_

data Term : Set where
  `_                      :  Id → Term
  ƛ_⇒_                    :  Id → Term → Term
  _∙_                     :  Term → Term → Term
  `zero                   :  Term
  `suc_                   :  Term → Term
  case_[zero⇒_|suc_⇒_]    :  Term → Term → Id → Term → Term
  μ_⇒_                    :  Id → Term → Term

two : Term
two = `suc `suc `zero

plus : Term
plus = μ "+" ⇒ ƛ "m" ⇒ ƛ "n" ⇒
         case ` "m"
           [zero⇒ ` "n"
           |suc "m" ⇒ `suc (` "+" ∙ ` "m" ∙ ` "n") ]

twoᶜ : Term
twoᶜ = ƛ "s" ⇒ ƛ "z" ⇒ ` "s" ∙ (` "s" ∙ ` "z")

plusᶜ : Term
plusᶜ = ƛ "m" ⇒ ƛ "n" ⇒ ƛ "s" ⇒ ƛ "z" ⇒
        ` "m" ∙ ` "s" ∙ (` "n" ∙ ` "s" ∙ ` "z")

sucᶜ : Term
sucᶜ = ƛ "n" ⇒ `suc (` "n")

mul : Term
mul = μ "*" ⇒ ƛ "m" ⇒ ƛ "n" ⇒
        case ` "m"
          [zero⇒ `zero
          |suc "m" ⇒ plus ∙ ` "n" ∙ ( ` "*" ∙ ` "m" ∙ ` "n" ) ]

mulᶜ : Term
mulᶜ = ƛ "m" ⇒ ƛ "n" ⇒ ƛ "s" ⇒ ƛ "z" ⇒
  ` "m" ∙ ( ƛ "x" ⇒ plusᶜ ∙ ` "n" ∙ ` "x" ∙ ` "s" ∙ ` "z" ) ∙ ` "z"

ƛ′_⇒_ : Term → Term → Term
ƛ′ (` x) ⇒ N  =  ƛ x ⇒ N
ƛ′ _ ⇒ _      =  ⊥-elim impossible
  where postulate impossible : ⊥

case′_[zero⇒_|suc_⇒_] : Term → Term → Term → Term → Term
case′ L [zero⇒ M |suc (` x) ⇒ N ]  =  case L [zero⇒ M |suc x ⇒ N ]
case′ _ [zero⇒ _ |suc _ ⇒ _ ]      =  ⊥-elim impossible
  where postulate impossible : ⊥

μ′_⇒_ : Term → Term → Term
μ′ (` x) ⇒ N  =  μ x ⇒ N
μ′ _ ⇒ _      =  ⊥-elim impossible
  where postulate impossible : ⊥

plus′ : Term
plus′ = μ′ + ⇒ ƛ′ m ⇒ ƛ′ n ⇒
          case′ m
            [zero⇒ n
            |suc m ⇒ `suc (+ ∙ m ∙ n) ]
  where
  +  =  ` "+"
  m  =  ` "m"
  n  =  ` "n"

mul′ : Term
mul′ = μ′ * ⇒ ƛ′ m ⇒ ƛ′ n ⇒
        case′ m
          [zero⇒ `zero
          |suc m ⇒ plus ∙ n ∙ ( * ∙ m ∙ n ) ]
  where
  *  =  ` "*"
  m  =  ` "m"
  n  =  ` "n"
