module Lists where

import Relation.Binary.PropositionalEquality as Eq
open Eq using (_≡_; refl; sym; trans; cong)
open Eq.≡-Reasoning
open import Data.Bool using (Bool; true; false; T; _∧_; _∨_; not)
open import Data.Nat using (ℕ; zero; suc; _+_; _*_; _∸_; _≤_; s≤s; z≤n)
open import Data.Nat.Properties using
  (+-assoc; +-identityˡ; +-identityʳ; *-assoc; *-identityˡ; *-identityʳ)
open import Relation.Nullary using (¬_; Dec; yes; no)
open import Data.Product using (_×_; ∃; ∃-syntax) renaming (_,_ to ⟨_,_⟩)
open import Data.Sum using (_⊎_; inj₁; inj₂)
open import Function using (_∘_)
open import Level using (Level)
open import Isomorphism using (_≃_; _⇔_; extensionality)
open import Inductions using (*-distrib-+; ∸-+-assoc; *-comm; +-comm)
open import Quantifiers using (∀-extensionality)
open import Data.Empty using (⊥; ⊥-elim)

data List (A : Set) : Set where
  [] : List A
  _∷_ : A → List A → List A

infixr 5 _∷_

_ : List ℕ
_ = 0 ∷ 1 ∷ 2 ∷ []

{-# BUILTIN LIST List #-}

pattern [_] z = z ∷ []
pattern [_,_] y z = y ∷ z ∷ []
pattern [_,_,_] x y z = x ∷ y ∷ z ∷ []
pattern [_,_,_,_] w x y z = w ∷ x ∷ y ∷ z ∷ []
pattern [_,_,_,_,_] v w x y z = v ∷ w ∷ x ∷ y ∷ z ∷ []
pattern [_,_,_,_,_,_] u v w x y z = u ∷ v ∷ w ∷ x ∷ y ∷ z ∷ []

_++_ : ∀ {A : Set} → List A → List A → List A
[] ++ ys = ys
(x ∷ xs) ++ ys = x ∷ (xs ++ ys)

infixr 5 _++_

_ : [ 0 , 1 , 2 ] ++ [ 3 , 4 ] ≡ [ 0 , 1 , 2 , 3 , 4 ]
_ =
  begin
    0 ∷ 1 ∷ 2 ∷ [] ++ 3 ∷ 4 ∷ []
  ≡⟨⟩
    0 ∷ (1 ∷ 2 ∷ [] ++ 3 ∷ 4 ∷ [])
  ≡⟨⟩
    0 ∷ 1 ∷ (2 ∷ [] ++ 3 ∷ 4 ∷ [])
  ≡⟨⟩
    0 ∷ 1 ∷ 2 ∷ ([] ++ 3 ∷ 4 ∷ [])
  ≡⟨⟩
    0 ∷ 1 ∷ 2 ∷ 3 ∷ 4 ∷ []
  ∎

++-assoc : ∀ {A : Set} → (xs ys zs : List A)
  → (xs ++ ys) ++ zs ≡ xs ++ (ys ++ zs)
++-assoc [] ys zs =
  begin
    ([] ++ ys) ++ zs
  ≡⟨⟩
    ys ++ zs
  ≡⟨⟩
    [] ++ (ys ++ zs)
  ∎
++-assoc (x ∷ xs) ys zs =
  begin
    (x ∷ xs ++ ys) ++ zs
  ≡⟨⟩
    x ∷ (xs ++ ys) ++ zs
  ≡⟨⟩
    x ∷ ((xs ++ ys) ++ zs)
  ≡⟨ cong (x ∷_) (++-assoc xs ys zs) ⟩
    x ∷ (xs ++ (ys ++ zs))
  ≡⟨⟩
    x ∷ xs ++ (ys ++ zs)
  ∎

++-identityˡ : ∀ {A : Set} (xs : List A) → [] ++ xs ≡ xs
++-identityˡ xs =
  begin
    [] ++ xs
  ≡⟨⟩
    xs
  ∎

++-identityʳ : ∀ {A : Set} (xs : List A) → xs ++ [] ≡ xs
++-identityʳ [] =
  begin
    [] ++ []
  ≡⟨⟩
    []
  ∎
++-identityʳ (x ∷ xs) =
  begin
    (x ∷ xs) ++ []
  ≡⟨⟩
    x ∷ (xs ++ [])
  ≡⟨ cong (x ∷_) (++-identityʳ xs) ⟩
    x ∷ xs
  ∎

length : ∀ {A : Set} → List A → ℕ
length [] = zero
length (_ ∷ xs) = suc (length xs)

_ : length [ 0 , 1 , 2 ] ≡ 3
_ =
  begin
    length (0 ∷ 1 ∷ 2 ∷ [])
  ≡⟨⟩
    suc (length (1 ∷ 2 ∷ []))
  ≡⟨⟩
    suc (suc (length (2 ∷ [])))
  ≡⟨⟩
    suc (suc (suc (length {ℕ} [])))
  ≡⟨⟩
    suc (suc (suc zero))
  ∎

length-++ : ∀ {A : Set} (xs ys : List A)
  → length (xs ++ ys) ≡ length xs + length ys
length-++ {A} [] ys =
  begin
    length ([] ++ ys)
  ≡⟨⟩
    length ys
  ≡⟨⟩
    length {A} [] + length ys
  ∎
length-++ (x ∷ xs) ys =
  begin
    length ((x ∷ xs) ++ ys)
  ≡⟨⟩
    suc (length (xs ++ ys))
  ≡⟨ cong suc (length-++ xs ys) ⟩
    suc (length xs + length ys)
  ≡⟨⟩
    length (x ∷ xs) + length ys
  ∎

reverse : ∀ {A : Set} → List A → List A
reverse [] = []
reverse (x ∷ xs) = reverse xs ++ [ x ]

_ : reverse [ 0 , 1 , 2 ] ≡ [ 2 , 1 , 0 ]
_ =
  begin
    reverse (0 ∷ 1 ∷ 2 ∷ [])
  ≡⟨⟩
    reverse (1 ∷ 2 ∷ []) ++ [ 0 ]
  ≡⟨⟩
    (reverse (2 ∷ []) ++ [ 1 ]) ++ [ 0 ]
  ≡⟨⟩
    ((reverse [] ++ [ 2 ]) ++ [ 1 ]) ++ [ 0 ]
  ≡⟨⟩
    (([] ++ [ 2 ]) ++ [ 1 ]) ++ [ 0 ]
  ≡⟨⟩
    (([] ++ 2 ∷ []) ++ 1 ∷ []) ++ 0 ∷ []
  ≡⟨⟩
    (2 ∷ [] ++ 1 ∷ []) ++ 0 ∷ []
  ≡⟨⟩
    2 ∷ ([] ++ 1 ∷ []) ++ 0 ∷ []
  ≡⟨⟩
    (2 ∷ 1 ∷ []) ++ 0 ∷ []
  ≡⟨⟩
    2 ∷ (1 ∷ [] ++ 0 ∷ [])
  ≡⟨⟩
    2 ∷ 1 ∷ ([] ++ 0 ∷ [])
  ≡⟨⟩
    2 ∷ 1 ∷ 0 ∷ []
  ≡⟨⟩
    [ 2 , 1 , 0 ]
  ∎

reverse-++-distrib : ∀ {A : Set} → (xs ys : List A)
  → reverse (xs ++ ys) ≡ reverse ys ++ reverse xs
reverse-++-distrib [] ys =
  begin
    reverse ([] ++ ys)
  ≡⟨⟩
    reverse ys
  ≡⟨ sym (++-identityʳ (reverse ys)) ⟩
    reverse ys ++ []
  ≡⟨⟩
    reverse ys ++ reverse []
  ∎
reverse-++-distrib (x ∷ xs) ys =
  begin
    reverse (x ∷ xs ++ ys)
  ≡⟨⟩
    reverse (xs ++ ys) ++ [ x ]
  ≡⟨ cong (_++ [ x ]) (reverse-++-distrib xs ys) ⟩
    (reverse ys ++ reverse xs) ++ [ x ]
  ≡⟨ ++-assoc (reverse ys) (reverse xs) [ x ] ⟩
    reverse ys ++ (reverse xs ++ [ x ])
  ≡⟨⟩
    reverse ys ++ reverse (x ∷ xs)
  ∎

reverse-extract : ∀ {A : Set} (xs : List A) (x : A)
  → reverse (xs ++ [ x ]) ≡ x ∷ reverse xs
reverse-extract [] x = refl
reverse-extract (x ∷ xs) y = cong (_++ [ x ]) (reverse-extract xs y)

reverse-involutive : ∀ {A : Set} {xs : List A}
  → reverse (reverse xs) ≡ xs
reverse-involutive {A} {[]} = refl
reverse-involutive {A} {x ∷ xs} =
  begin
      reverse (reverse xs ++ [ x ])
  ≡⟨ reverse-extract (reverse xs) x ⟩
      (x ∷ reverse (reverse xs))
  ≡⟨ cong (x ∷_) (reverse-involutive {A} {xs}) ⟩
      (x ∷ xs)
  ∎

shunt : ∀ {A : Set} → List A → List A → List A
shunt [] ys = ys
shunt (x ∷ xs) ys = shunt xs (x ∷ ys)

shunt-reverse : ∀ {A : Set} (xs ys : List A)
  → shunt xs ys ≡ reverse xs ++ ys
shunt-reverse [] ys =
  begin
    shunt [] ys
  ≡⟨⟩
    ys
  ≡⟨⟩
    reverse [] ++ ys
  ∎
shunt-reverse (x ∷ xs) ys =
  begin
    shunt (x ∷ xs) ys
  ≡⟨⟩
    shunt xs (x ∷ ys)
  ≡⟨ shunt-reverse xs (x ∷ ys) ⟩
    reverse xs ++ (x ∷ ys)
  ≡⟨⟩
    reverse xs ++ ([ x ] ++ ys)
  ≡⟨ sym (++-assoc (reverse xs) [ x ] ys) ⟩
    (reverse xs ++ [ x ]) ++ ys
  ≡⟨⟩
    reverse (x ∷ xs) ++ ys
  ∎

reverse′ : ∀ {A : Set} → List A → List A
reverse′ xs = shunt xs []

reverses : ∀ {A : Set} (xs : List A)
  → reverse′ xs ≡ reverse xs
reverses xs =
  begin
    reverse′ xs
  ≡⟨⟩
    shunt xs []
  ≡⟨ shunt-reverse xs [] ⟩
    reverse xs ++ []
  ≡⟨ ++-identityʳ (reverse xs) ⟩
    reverse xs
  ∎

_ : reverse′ [ 0 , 1 , 2 ] ≡ [ 2 , 1 , 0 ]
_ =
  begin
    reverse′ (0 ∷ 1 ∷ 2 ∷ [])
  ≡⟨⟩
    shunt (0 ∷ 1 ∷ 2 ∷ []) []
  ≡⟨⟩
    shunt (1 ∷ 2 ∷ []) (0 ∷ [])
  ≡⟨⟩
    shunt (2 ∷ []) (1 ∷ 0 ∷ [])
  ≡⟨⟩
    shunt [] (2 ∷ 1 ∷ 0 ∷ [])
  ≡⟨⟩
    2 ∷ 1 ∷ 0 ∷ []
  ∎

map : ∀ {A B : Set} → (A → B) → List A → List B
map f [] = []
map f (x ∷ xs) = f x ∷ map f xs

_ : map suc [ 0 , 1 , 2 ] ≡ [ 1 , 2 , 3 ]
_ =
  begin
    map suc (0 ∷ 1 ∷ 2 ∷ [])
  ≡⟨⟩
    suc 0 ∷ map suc (1 ∷ 2 ∷ [])
  ≡⟨⟩
    suc 0 ∷ suc 1 ∷ map suc (2 ∷ [])
  ≡⟨⟩
    suc 0 ∷ suc 1 ∷ suc 2 ∷ map suc []
  ≡⟨⟩
    suc 0 ∷ suc 1 ∷ suc 2 ∷ []
  ≡⟨⟩
    1 ∷ 2 ∷ 3 ∷ []
  ∎

sucs : List ℕ → List ℕ
sucs = map suc

_ : sucs [ 0 , 1 , 2 ] ≡ [ 1 , 2 , 3 ]
_ =
  begin
    sucs [ 0 , 1 , 2 ]
  ≡⟨⟩
    map suc [ 0 , 1 , 2 ]
  ≡⟨⟩
    [ 1 , 2 , 3 ]
  ∎

map-compose : ∀ {A B C : Set} {f : A → B} {g : B → C}
  → map (g ∘ f) ≡ map g ∘ map f
map-compose {A} {B} {C} {f} {g} = extensionality (lemma f g)
  where
    lemma : ∀ {A B C : Set} (f : A → B) (g : B → C) (xs : List A)
       → map (g ∘ f) xs ≡ (map g ∘ map f) xs
    lemma f g [] = refl
    lemma f g (x ∷ xs) = cong ((g ∘ f) x ∷_) (lemma f g xs)

map-++-commute : ∀ {A B : Set} {f : A → B} {xs ys : List A}
  → map f (xs ++ ys) ≡ map f xs ++ map f ys
map-++-commute {A} {B} {f} {[]} {ys} = refl
map-++-commute {A} {B} {f} {x ∷ xs} {ys} = 
  cong (f x ∷_) (map-++-commute {A} {B} {f} {xs} {ys})

data Tree (A B : Set) : Set where
  leaf : A → Tree A B
  node : Tree A B → B → Tree A B → Tree A B

map-Tree : ∀ {A B C D : Set} → (A → C) → (B → D) → Tree A B → Tree C D
map-Tree f g (leaf x) = leaf (f x)
map-Tree f g (node t x t′) = node (map-Tree f g t) (g x) (map-Tree f g t′)

foldr : ∀ {A B : Set} → (A → B → B) → B → List A → B
foldr _⊗_ b [] = b
foldr _⊗_ b (x ∷ xs) = x ⊗ foldr _⊗_ b xs

_ : foldr _+_ 0 [ 1 , 2 , 3 , 4 ] ≡ 10
_ =
  begin
    foldr _+_ 0 (1 ∷ 2 ∷ 3 ∷ 4 ∷ [])
  ≡⟨⟩
    1 + foldr _+_ 0 (2 ∷ 3 ∷ 4 ∷ [])
  ≡⟨⟩
    1 + (2 + foldr _+_ 0 (3 ∷ 4 ∷ []))
  ≡⟨⟩
    1 + (2 + (3 + foldr _+_ 0 (4 ∷ [])))
  ≡⟨⟩
    1 + (2 + (3 + (4 + foldr _+_ 0 [])))
  ≡⟨⟩
    1 + (2 + (3 + (4 + 0)))
  ∎

sum : List ℕ → ℕ
sum = foldr _+_ 0

_ : sum [ 1 , 2 , 3 , 4 ] ≡ 10
_ =
  begin
    sum [ 1 , 2 , 3 , 4 ]
  ≡⟨⟩
    foldr _+_ 0 [ 1 , 2 , 3 , 4 ]
  ≡⟨⟩
    10
  ∎

product : List ℕ → ℕ
product = foldr _*_ 1

foldr-++ : ∀ {A B : Set} (_⊗_ : A → B → B) (e : B) (xs ys : List A) →
  foldr _⊗_ e (xs ++ ys) ≡ foldr _⊗_ (foldr _⊗_ e ys) xs
foldr-++ _⊗_ e [] ys = refl
foldr-++ _⊗_ e (x ∷ xs) ys = cong (x ⊗_) (foldr-++ _⊗_ e xs ys)

map-is-foldr : ∀ {A B : Set} {f : A → B} →
  map f ≡ foldr (λ x xs → f x ∷ xs) []
map-is-foldr {A} {B} {f} = extensionality lemma
  where
    lemma : ∀ {A B : Set} {f : A → B} (xs : List A) →
      map f xs ≡ foldr (λ x xs → f x ∷ xs) [] xs
    lemma [] = refl
    lemma {A} {B} {f} (x ∷ xs) = cong (f x ∷_) (lemma xs)

fold-Tree : ∀ {A B C : Set} → (A → C) → (C → B → C → C) → Tree A B → C
fold-Tree f g (leaf x) = f x
fold-Tree f g (node t x t′) = g (fold-Tree f g t) x (fold-Tree f g t′)

map-is-fold-Tree : ∀ {A B C D : Set} {f : A → C} {g : B → D} →
  map-Tree f g ≡ fold-Tree {A} {B} {Tree C D} 
                 (λ x → leaf (f x))
                 (λ lf x rt → node lf (g x) rt)
map-is-fold-Tree = extensionality lemma
  where
    lemma : ∀ {A B C D : Set} {f : A → C} {g : B → D} (xs : Tree A B) →
      map-Tree f g xs ≡ fold-Tree {A} {B} {Tree C D}
                        (λ x → leaf (f x))
                        (λ lf x rt → node lf (g x) rt) xs
    lemma (leaf x) = refl
    lemma {A} {B} {C} {D} {f} {g} (node lf x rt)
                                  rewrite lemma {A} {B} {C} {D} {f} {g} lf
                                | lemma {A} {B} {C} {D} {f} {g} rt = refl
